src/lib/Axioms.v
@@ -6,6 +6,8 @@ Require Coq.Logic.Epsilon.
 Require Logic.Classical_Pred_Type.
 Require Import Coq.Logic.ProofIrrelevance.
 Require Import Coq.Logic.ClassicalEpsilon.
+Require Import Coq.Logic.IndefiniteDescription.
+
 
 Set Implicit Arguments.
 
@@ -43,3 +45,12 @@ Ltac nean H := eapply not_ex_all_not_help in H; red in H.
 Definition proof_irrelevance := proof_irrelevance.
 Definition excluded_middle_informative := excluded_middle_informative.
 Definition choice := choice.
+
+Lemma dependent_functional_choice (A : Type) (B : A -> Type) :
+  forall R : forall x : A, B x -> Prop,
+    (forall x : A, exists y : B x, R x y) ->
+    (exists f : (forall x : A, B x), forall x : A, R x (f x)).
+Proof.
+  eapply ChoiceFacts.non_dep_dep_functional_choice.
+  clear. exact functional_choice.
+Qed.
